Etch/StreamFusion/Main.lean
@@ -1,0 +1,341 @@
+import Std.Data.RBMap
+import Std.Data.HashMap
+
+import Etch.StreamFusion.Stream
+import Etch.StreamFusion.Multiply
+import Etch.StreamFusion.Traversals
+
+open Std (RBMap HashMap)
+open Etch.Verification
+open SStream
+open OfStream ToStream
+
+-- deprecated
+@[inline] def vecStream' (num : Nat) := stream $ Array.range num |>.map fun n => (n,n)
+
+@[inline] def vecStream (num : Nat) :=
+  let v : Vec ℕ num := ⟨Array.range num, Array.size_range⟩
+  stream $ Level.mk v v
+
+--@[inline] def floatVecStream (num : Nat) :=
+--  let is : Vec ℕ num := ⟨Array.range num, Array.size_range⟩
+--  let vs : FloatVec num := ⟨Array.range num |>.toList.map (fun x => x.toFloat) |>.toFloatArray, by sorry⟩
+--  stream $ (is, vs)
+
+-- adjusts size so that there are ~num non-zero entries
+@[macro_inline]
+def mat (num : Nat) :=
+  let m1 : Array (ℕ × Array (ℕ × ℕ)) :=
+    Array.range (2*num).sqrt |>.map (.+1) |>.map $ fun n =>
+      (n, Array.range n |>.map fun m => (m, m+10))
+  stream m1
+
+@[macro_inline]
+def mat' (num : Nat) :=
+  let m1 : Array (ℕ × Array (ℕ × ℕ)) :=
+    Array.range num |>.map (.+1) |>.map $ fun n =>
+      (n, Array.range n |>.map fun m => (m, m+10))
+  stream m1
+
+def time (s : String) (m : Unit → IO α) : IO α := do
+  let t0 ← IO.monoMsNow
+  let v ← m ()
+  let t1 ← IO.monoMsNow
+  IO.println s!"[{s}] time: {t1-t0}"
+  pure v
+
+namespace test
+-- these tests need to be separate defs for profile legibility
+def baseline (num : Nat) : IO Unit := do
+  IO.println "-----------"
+  let arr_ := Array.range num
+  --let arr := arr_ |>.map fun n => (n,n)
+  time "baseline (forIn) vec sum" fun _ =>
+    for _ in [0:10] do
+      let mut m := 0
+      for i in arr_ do
+        m := m + i
+      IO.println s!"{m}"
+
+def vecSum_slow (num : Nat) : IO Unit := do
+  IO.println "-----------"
+  let s := contract $ vecStream num
+  time "vec sum (slower)" fun _ =>
+    for _ in [0:10] do
+      let x : ℕ := eval s
+      IO.println s!"{x}"
+
+def vecSum (num : Nat) : IO Unit := do
+  IO.println "-----------"
+  let s := contract $ vecStream num
+  time "vec sum" fun _ =>
+    for _ in [0:10] do
+      let x : ℕ := eval s
+      IO.println s!"{x}"
+
+--def testFloat (num : Nat) : IO Unit := do
+--  IO.println "-----------"
+--  let s := contract $ floatVecStream num
+--  time "float stream" fun _ =>
+--    for _ in [0:10] do
+--      let x : Float := eval s
+--      IO.println s!"{x}"
+
+def vecMul (num : Nat) : IO Unit := do
+  IO.println "-----------"
+  let v := vecStream num
+  let v' := vecStream num |>.map fun _ => 1
+  let s := v * v'
+  time "vec mul" fun _ =>
+    for _ in [0:10] do
+      let x : Array ℕ × Array ℕ := eval s
+      IO.println s!"{x.1.size}"
+  pure ()
+
+abbrev Map a [Ord a] b := RBMap a b Ord.compare
+
+def vecMul_rb (num : Nat) : IO Unit := do
+  IO.println "-----------"
+  let v := vecStream num
+  let s := v * (v.map fun _ => 1)
+  time "vec mul rb" fun _ =>
+    for _ in [0:10] do
+      let x : RBMap ℕ ℕ Ord.compare := eval s
+      IO.println s!"{x.1.size}"
+  pure ()
+
+def vecMul_hash (num : Nat) : IO Unit := do
+  IO.println "-----------"
+  let v := vecStream num
+  let v' := vecStream num |>.map fun _ => 1
+  let s := v * v'
+  time "vec mul hash" fun _ =>
+    for _ in [0:10] do
+      let x : HashMap ℕ ℕ := eval s
+      IO.println s!"{x.1.size}"
+  pure ()
+
+def vecMulSum (num : Nat) : IO Unit := do
+  IO.println "-----------"
+  let v := vecStream num
+  let v' := vecStream num |>.map fun _ => 1
+  let s := contract $ v * v'
+  time "vec mul sum" fun _ =>
+    for _ in [0:10] do
+      let x : ℕ := eval s
+      IO.println s!"{x}"
+  pure ()
+
+-- todo: this has allocation and other perf issues
+def vecMulSum3 (num : Nat) : IO Unit := do
+  IO.println "-----------"
+  let v := vecStream num
+  let v₁ := vecStream num |>.map fun _ => 1
+  let v₂ := vecStream num |>.map fun _ => 1
+  let s := contract $ v * v₁ * v₂
+  time "vec mul 3 sum slow?" fun _ =>
+    for _ in [0:10] do
+      let x : ℕ := eval s
+      IO.println s!"{x}"
+  pure ()
+
+def matSum (num : Nat) : IO Unit := do
+  IO.println "-----------"
+  let s := contract2 $ mat num
+  time "matrix sum" fun _ =>
+    for _ in [0:10] do
+      let x : ℕ := eval s
+      IO.println s!"{x}"
+
+-- todo: not inlining!
+def matProdSum (num : Nat) : IO Unit := do
+  IO.println "-----------"
+  let m := mat num
+  let s := contract2 $ m * m
+  time "matrix prod sum" fun _ =>
+    for _ in [0:10] do
+      let x : ℕ := eval s
+      IO.println s!"{x}"
+
+def _root_.Nat.cubeRoot (n : Nat) : Nat :=
+  if n ≤ 1 then n else
+  iter n (n / 2)
+where
+  iter (n guess : Nat) : Nat :=
+    let next := (2*guess + n / (guess * guess)) / 3
+    if _h : next < guess then
+      iter n next
+    else
+      guess
+termination_by iter guess => guess
+
+@[macro_inline]
+def aMatMul (n : Nat) : ℕ →ₛ ℕ →ₛ Unit →ₛ ℕ :=
+  let m := mat' (4*n).cubeRoot;
+  let m' := mat' (4*n).cubeRoot;
+  let m1 : ℕ →ₛ ℕ →  ℕ →ₛ ℕ := map expand m
+  let m2 : ℕ →ₛ ℕ →ₛ ℕ → ℕ := map (map expand) m'
+  let s  : ℕ →ₛ ℕ →ₛ ℕ →ₛ ℕ := m1 * m2
+  map (map contract) $ s
+
+def matMultiplySum (num : Nat) : IO Unit := do
+  IO.println "-----------"
+  let s := contract2 $ aMatMul num
+  time "matrix multiply (inner-product) sum" fun _ =>
+    for _ in [0:10] do
+      let x : ℕ := eval s
+      IO.println s!"{x}"
+
+def matMultiply1 (num : Nat) : IO Unit := do
+  IO.println "-----------"
+  let s := aMatMul num
+  time "matrix multiply (inner-product) arrays" fun _ =>
+    for _ in [0:10] do
+      let x : Array ℕ × Array (Array ℕ × Array ℕ) := eval s
+      IO.println s!"{x.1.size}"
+
+-- todo: this isn't being inlined correctly
+def matMultiply2 (num : Nat) : IO Unit := do
+  IO.println "-----------"
+  let s := aMatMul num
+  time "matrix multiply (inner-product) array hashmap" fun _ =>
+    for _ in [0:10] do
+      let y : Array ℕ × Array (HashMap ℕ ℕ) := eval s
+      IO.println s!"{y.2.size}"
+
+def matMultiply3 (num : Nat) : IO Unit := do
+  IO.println "-----------"
+  let s := aMatMul num
+  time "matrix multiply (inner-product) array rbmap" fun _ =>
+    for _ in [0:10] do
+      let y : Array ℕ × Array (RBMap ℕ ℕ Ord.compare) := eval s
+      IO.println s!"{y.2.size}"
+
+def baselineRB (num : Nat) : IO Unit := do
+  IO.println "-----------"
+  let arr_ := Array.range num
+  let map := RBMap.ofList (arr_.toList.map fun i => (i, 1)) Ord.compare
+  let map' : Tree' ℕ ℕ := map.1.map fun (i,v) => (i, Side.no, v)
+  let test (map : RBMap ℕ ℕ Ord.compare) := do
+    time "forIn vec * rbmap sum" fun _ => -- about 10x slower than vecMulSum
+      for _ in [0:10] do
+        let mut m := 0
+        for i in arr_ do
+          m := m + i * (map.toFn i)
+        IO.println s!"{m}"
+    time "forIn rbmap * vec sum" fun _ => -- about 5x slower than vecMulSum
+      for _ in [0:10] do
+        let mut m := 0
+        for (i,v) in map do
+          m := m + arr_.get! i * v
+        IO.println s!"{m}"
+    time "RBMap.map" fun _ => do -- baseline
+      let mut map := map.1
+      for _ in [0:10] do
+        map := map.map fun x => (x.1, x.2 * 2)
+        IO.println s!"{map.look}"
+    -- about 1.8x slower than baseline. no stack. allocation
+    time "tmap" fun _ => do
+      let mut map := map.1
+      for _ in [0:10] do
+        map := tmap (t := map) fun b => b*2
+        IO.println s!"{map.look}"
+    -- about 1.5x slower than baseline. no stack. no allocation
+    time "tmap fbip" fun _ => do
+      let mut map : Tree' ℕ ℕ := map'
+      for _ in [0:10] do
+        map := tmap' (t := map) fun b => b*2
+        IO.println s!"{let (i, _, x) := map.look; (i,x)}"
+  test map
+
+unsafe def testRB (args : List String) : IO Unit := do
+  let num := (args[0]!).toNat?.getD 1000
+  IO.println s!"test of size {num}"
+  IO.println "starting"
+
+  test.baselineRB num
+
+end test
+
+unsafe def testAll (args : List String) : IO Unit := do
+  let num := (args[0]!).toNat?.getD 1000
+  IO.println s!"test of size {num}"
+  IO.println "starting"
+
+  test.baseline num
+  test.vecSum num
+  test.vecMulSum num      -- ideally about 2x vecSum
+  test.vecMulSum3 num      -- ideally about 2x vecSum
+  test.vecMul num         -- ideally about 1x vecMulSum (currently 3x slower, but that's almost all Array.push. try pre-allocating?)
+  test.matSum num         -- ideally about 1x vecSum
+  test.matProdSum num     -- ... 2x matSum
+  test.matMultiplySum num
+  test.matMultiply1 num
+  test.matMultiply2 num
+  test.matMultiply3 num
+
+unsafe def testSome (args : List String) : IO Unit := do
+  let num := (args[0]!).toNat?.getD 1000
+  IO.println s!"test of size {num}"
+  IO.println "starting"
+
+  test.baseline num
+  test.vecSum num
+  test.vecMulSum num
+  test.vecMulSum3 num
+  test.vecMul num
+
+  --test.matProdSum num
+
+  --test.vecMul_rb num
+  test.matMultiply1 num
+  --test.matMultiply3 num
+
+unsafe def _root_.main := testSome
+
+section appendix
+-- simple inline/specialize example
+@[inline] unsafe def myArrayLoop {β : Type v} [Add β] (as : Array β) (b : β) : β :=
+  let sz := USize.ofNat as.size
+  let rec @[specialize] loop (i : USize) (b : β) : β :=
+    if i < sz then
+      let a := as.uget i lcProof
+      loop (i+1) (b + a)
+    else
+      b
+  loop 0 b
+
+def test1Floats (num : Nat) : IO Unit := do
+  IO.println "-----------"
+  let arr_ := Array.range num |>.map Nat.toFloat |>.toList.toFloatArray
+  --let arr := arr_ |>.map fun n => (n,n)
+  time "lean forIn FloatArray" fun _ =>
+    for _ in [0:10] do
+      let mut m := 0
+      for i in arr_ do
+        m := m + i
+      IO.println s!"{m}"
+
+unsafe def test2 (num : Nat) : IO Unit := do
+  IO.println "-----------"
+  let arr := Array.range num
+  time "myForIn" fun _ =>
+    for _ in [0:10] do
+      let x := myArrayLoop arr 0
+      IO.println s!"{x}"
+
+-- IR playground
+section compiler_trace
+@[inline]
+def str1 := vecStream 10
+--set_option trace.compiler.inline true
+--set_option trace.compiler.specialize true
+--set_option trace.compiler.stage2 true
+--def thetest' : ℕ := eval (contract (vecStream' 10)) --
+@[noinline] def dup (x : α) := (x, x) example (x : ℕ) := let (a, _) := dup x; a
+--def multest_ := let str1 := vecStream' 10; eval (contract (str1 * str1))
+--def foo (n : ℕ) := let s := contract2 (mat n); eval s
+unsafe example := myArrayLoop #[] 0
+end compiler_trace
+
+end appendix
